wip: surpassing elements

Pearls/SurpassingElements.dfy
@@ -1,108 +1,265 @@
 include "./SeqFunctions.dfy"
 module SurpassingProblem {
-    import opened SeqFunctions
-    function Tails<T>(xs: seq<T>): seq<seq<T>> {
-        if xs == [] then
-            []
-        else
-            [xs]+Tails(xs[1..])
-    }
+  import opened SeqFunctions
+  function Tails<T>(xs: seq<T>): seq<seq<T>>
+    ensures forall xxs :: xxs in Tails(xs) ==> |xs| > 0
+  {
+    if xs == [] then
+      []
+    else
+      [xs]+Tails(xs[1..])
+  }
 
-    function scount<T>(x: T, xs: seq<T>, cpm: (T,T) -> bool): nat {
-        |Filter(y => cpm(x,y) ,xs)|
-    }
+  lemma TailsHas<T(==)>(xs: seq<T>, i: nat)
+    requires 0 <= i < |xs|
+    ensures xs[i..] in Tails(xs)
+  {
+    if i == 0 {
 
-    lemma LemmaTailsConcat<T>(xs: seq<T>, ys: seq<T>)
-        ensures Tails(xs+ys) == Map(xxs => xxs+ys, Tails(xs))+Tails(ys)
+    }else{
+      // assert xs[]
+      TailsHas(xs[1..], i-1);
+
+    }
+  }
+
+  lemma TailsHasAllSlices<T(==)>(xs: seq<T>)
+    ensures forall i :: 0 <= i < |xs| ==> xs[i..] in Tails(xs)
+  {
+
+    forall i | 0 <= i < |xs|
+      ensures xs[i..] in Tails(xs)
     {
-        if xs == [] {
-            assert xs+ys == ys;
-            assert Tails(xs) == [];
+      TailsHas(xs,i);
+    }
+  }
 
-            assert Tails(xs+ys) == Map(xxs => xxs+ys,Tails(xs))+Tails(ys);
-        }else if |xs| == 1 {
-    
-            assert Tails(xs+ys) == Map(xxs => xxs+ys,Tails(xs))+Tails(ys);
-        }else{
-            assert xs==[xs[0]]+xs[1..];
-            assert (xs+ys)[1..] == xs[1..]+ys;
-            LemmaTailsConcat(xs[1..], ys);
+  function scount<T>(x: T, xs: seq<T>, cpm: (T,T) -> bool): nat {
+    |Filter(y => cpm(x,y) ,xs)|
+  }
 
-            assert Tails(xs+ys) == Map(xxs => xxs+ys,Tails(xs))+Tails(ys);
+  lemma ScountHasLarger<T>(x: T, xs: seq<T>, cpm: (T,T) -> bool)
+    ensures forall z :: z in Filter(y => cpm(x, y), xs) ==> cpm(x, z)
+  {}
+
+  lemma LemmaTailsConcat<T>(xs: seq<T>, ys: seq<T>)
+    ensures Tails(xs+ys) == Map(xxs => xxs+ys, Tails(xs))+Tails(ys)
+  {
+    if xs == [] {
+      assert xs+ys == ys;
+      assert Tails(xs) == [];
+
+      assert Tails(xs+ys) == Map(xxs => xxs+ys,Tails(xs))+Tails(ys);
+    }else if |xs| == 1 {
+
+      assert Tails(xs+ys) == Map(xxs => xxs+ys,Tails(xs))+Tails(ys);
+    }else{
+      assert xs==[xs[0]]+xs[1..];
+      assert (xs+ys)[1..] == xs[1..]+ys;
+      LemmaTailsConcat(xs[1..], ys);
+
+      assert Tails(xs+ys) == Map(xxs => xxs+ys,Tails(xs))+Tails(ys);
+    }
+  }
+
+  lemma LemmaScountConcat<T>(xs: seq<T>, ys: seq<T>, z: T, cmp: (T,T) -> bool)
+    ensures scount(z, xs+ys, cmp) == scount(z,xs,cmp) + scount(z,ys,cmp)
+  {
+    if xs == [] {
+      assert xs+ys == ys;
+      assert scount(z, xs+ys, cmp) == scount(z,xs,cmp) + scount(z,ys,cmp);
+    }else if |xs| == 1 {
+      assert scount(z, xs+ys, cmp) == scount(z,xs,cmp) + scount(z,ys,cmp);
+    }else{
+      assert xs==[xs[0]]+xs[1..];
+      assert (xs+ys)[1..] == xs[1..]+ys;
+      LemmaScountConcat(xs[1..], ys, z, cmp);
+
+      assert scount(z, xs+ys, cmp) == scount(z,xs,cmp) + scount(z,ys,cmp);
+    }
+  }
+
+  function maxNat(m: nat, a: nat): nat {
+    if a > m then a else m
+  }
+
+  function maximum(xs: seq<nat>): nat
+    requires |xs| > 0
+  {
+    FoldRight(maxNat, xs, xs[0])
+  }
+
+  lemma LemmaFoldRightMax(xs: seq<nat>, init: nat)
+    ensures forall x :: x in xs ||x in {init} ==> FoldRight(maxNat, xs, init) >= x
+  {
+    if xs == [] {
+
+    }else if |xs| == 1 {
+
+    }else{
+      assert xs == [xs[0]] + xs[1..];
+
+    }
+  }
+
+  lemma LemmaMaximum(xs: seq<nat>)
+    requires |xs| > 0
+    ensures forall x:: x in xs ==> maximum(xs) >= x
+  {
+    if |xs| == 1{
+
+    }else{
+      LemmaFoldRightMax(xs, xs[0]);
+    }
+  }
+  lemma LemmaMaximumConcat(xs: seq<nat>, ys: seq<nat>)
+    requires |ys| > 0
+    requires |xs| > 0
+    ensures maximum(xs+ys) == maxNat(maximum(xs), maximum(ys))
+  {
+    if |xs| == 1 {
+
+    }else{
+      LemmaMaximumConcat(xs[1..], ys);
+    }
+  }
+
+  lemma LemmaMaximumIn(xs: seq<nat>)
+    requires |xs| > 0
+    ensures maximum(xs) in xs
+  {
+    if |xs| == 1 {
+      calc {
+        maximum(xs);
+        FoldRight(maxNat, xs, xs[0]);
+        maxNat(xs[0], FoldRight(maxNat, xs[1..], xs[0]));
+        maxNat(xs[0], FoldRight(maxNat, [], xs[0]));
+        maxNat(xs[0], xs[0]);
+        xs[0];
+      }
+      assert maximum(xs) in xs;
+    }else{
+      assert xs == [xs[0]]+xs[1..];
+      LemmaMaximumIn(xs[1..]);
+      LemmaFoldRightDistributesOverConcat(maxNat,xs[0], [xs[0]],xs[1..]);
+
+      calc {
+        maximum(xs);
+        FoldRight(maxNat, xs, xs[0]);
+        FoldRight(maxNat, [xs[0]], FoldRight(maxNat, xs[1..], xs[0]));
+        // maxNat(xs[0], FoldRight(maxNat, xs[1..], xs[0]));
+      }
+      if xs[0] >  maximum(xs[1..]) {
+
+        assert maximum(xs) in xs;
+      }else{
+
+        assert maximum(xs) in xs;
+      }
+      assert maximum(xs) in xs;
+
+    }
+  }
+
+  ghost function maxScount(xs: seq<int>): nat
+    requires |xs| > 0
+  {
+    ThereIsAMaxScount(xs);
+    var m :| 0 <= m < |xs| && forall i :: 0 <= i < |xs| ==> scount(xs[m..][0], xs[m..][1..], (a,b) => a <b) >= scount(xs[i..][0], xs[i..][1..], (a,b) => a <b);
+    scount(xs[m..][0], xs[m..][1..], (a,b) => a < b)
+  }
+
+  function msc(xs: seq<int>): nat
+    requires |xs| > 0
+  {
+    var zzs := Map((zs) => assume |zs| > 0;
+                     scount(zs[0], zs[1..], (a,b)=> a < b), Tails(xs));
+    maximum(zzs)
+  }
+
+  lemma {:isolate_assertions} mscIsMaximum(xs: seq<int>)
+    requires |xs| > 0
+    ensures msc(xs) == maxScount(xs)
+  {
+    if |xs| == 1 {
+      assert xs[1..] == [];
+      assert Tails(xs) == [xs] + Tails(xs[1..]);
+      assert Tails(xs) == [xs];
+      assert Filter(xxs => |xxs| > 0, Tails(xs)) == [xs];
+      assert scount(xs[0..][0], xs[0..][1..], (a,b) => a <b) == scount(xs[0], xs[1..], (a,b) => a <b);
+      ThereIsAMaxScount(xs);
+      var m :| 0 <= m < |xs| && forall i :: 0 <= i < |xs| ==> scount(xs[m..][0], xs[m..][1..], (a,b) => a <b) >= scount(xs[i..][0], xs[i..][1..], (a,b) => a <b);
+      assert m == 0;
+      assert msc(xs) == maxScount(xs);
+    }else{
+      mscIsMaximum(xs[1..]);
+      assert xs == [xs[0]]+xs[1..];
+      assert msc(xs) == maxScount(xs);
+    }
+  }
+
+  lemma ThereIsAMaxScount(xs: seq<int>)
+    requires |xs| > 0
+    ensures exists m :: 0 <= m < |xs| && forall i :: 0 <= i < |xs| ==> scount(xs[m..][0], xs[m..][1..], (a,b) => a <b) >= scount(xs[i..][0], xs[i..][1..], (a,b) => a <b)
+  {
+    if |xs| == 1 {
+      assert xs[1..] == [];
+      assert scount(xs[0..][0], xs[0..][1..], (a,b) => a <b) == scount(xs[0], xs[1..], (a,b) => a <b);
+      assert exists m :: 0 <= m < |xs| && forall i :: 0 <= i < |xs| ==> scount(xs[m..][0], xs[m..][1..], (a,b) => a <b) >= scount(xs[i..][0], xs[i..][1..], (a,b) => a <b);
+    }else{
+      ThereIsAMaxScount(xs[1..]);
+      var m :| 0 <= m < |xs[1..]| && forall i :: 0 <= i < |xs[1..]| ==> scount(xs[1..][m..][0], xs[1..][m..][1..], (a,b) => a <b) >= scount(xs[1..][i..][0], xs[1..][i..][1..], (a,b) => a <b);
+      assert xs == [xs[0]]+xs[1..];
+      assert xs[1..][m..] == xs[m+1..];
+      assert scount(xs[0..][0], xs[0..][1..], (a,b) => a <b) == scount(xs[0], xs[1..], (a,b) => a <b);
+      assert forall i :: 0 <= i < |xs[1..]| ==> xs[1..][i..] == xs[i+1..];
+      if scount(xs[0], xs[1..], (a,b) => a <b) > scount(xs[1..][m..][0], xs[1..][m..][1..], (a,b) => a <b) {
+
+        forall i | 0 <= i < |xs|
+          ensures scount(xs[0], xs[1..], (a,b) => a <b) >= scount(xs[i..][0], xs[i..][1..], (a,b) => a <b);
+        {
+          if i == 0 {
+          }else{
+            assert xs[i..] == xs[1..][(i-1)..];
+          }
+
         }
-    }
-
-    lemma LemmaScountConcat<T>(xs: seq<T>, ys: seq<T>, z: T, cmp: (T,T) -> bool)
-        ensures scount(z, xs+ys, cmp) == scount(z,xs,cmp) + scount(z,ys,cmp)
-    {
-        if xs == [] {
-            assert xs+ys == ys;
-            assert scount(z, xs+ys, cmp) == scount(z,xs,cmp) + scount(z,ys,cmp);
-        }else if |xs| == 1 {
-            assert scount(z, xs+ys, cmp) == scount(z,xs,cmp) + scount(z,ys,cmp);
-        }else{
-            assert xs==[xs[0]]+xs[1..];
-            assert (xs+ys)[1..] == xs[1..]+ys;
-            LemmaScountConcat(xs[1..], ys, z, cmp);
-
-            assert scount(z, xs+ys, cmp) == scount(z,xs,cmp) + scount(z,ys,cmp);
+      }else{
+        forall i | 0 <= i < |xs|
+          ensures scount(xs[m+1..][0], xs[m+1..][1..], (a,b) => a <b) >= scount(xs[i..][0], xs[i..][1..], (a,b) => a <b);
+        {
+          if i == 0 {
+            assert scount(xs[m+1..][0], xs[m+1..][1..], (a,b) => a <b) >= scount(xs[0], xs[1..], (a,b) => a <b);
+          }else{
+            assert xs[i..] == xs[1..][(i-1)..];
+            assert scount(xs[i..][0], xs[i..][1..], (a,b) => a <b) == scount(xs[1..][(i-1)..][0], xs[1..][i-1..][1..], (a,b) => a <b);
+            assert scount(xs[m+1..][0], xs[m+1..][1..], (a,b) => a <b) >= scount(xs[i..][0], xs[i..][1..], (a,b) => a <b);
+          }
         }
+      }
+      assert exists m :: 0 <= m < |xs| && forall i :: 0 <= i < |xs| ==> scount(xs[m..][0], xs[m..][1..], (a,b) => a <b) >= scount(xs[i..][0], xs[i..][1..], (a,b) => a <b);
+
     }
+  }
 
-    function maxNat(m: nat, a: nat): nat {
-        if a > m then a else m
-    }
+  // lemma mscHasAllGreaterSlices(xs: seq<int>, cpm: (int,int) -> bool, i: nat)
+  //     requires 0 <= i < |xs|
+  //     requires |xs[i..]| > 0
+  //     requires forall z :: z in Filter(y => cpm(xs[i..][0], z), xs[i..]) ==> cpm(xs[i..][0], z)
+  // {}
 
-    function maximum(xs: seq<nat>): nat
-        requires |xs| > 0
-    {
-        FoldRight(maxNat, xs, xs[0])
-    }
+  function table(xs: seq<int>): seq<(int, nat)>
+    requires |xs| > 1
+  {
+    Map((zs) => assume |zs| > 0;
+          (zs[0], scount(zs[0], zs[1..], (a,b)=> a < b)), Filter(xxs => |xxs| > 0, Tails(xs)))
+  }
 
-    lemma LemmaFoldRightMax(xs: seq<nat>, init: nat)
-        ensures forall x :: x in xs ||x in {init} ==> FoldRight(maxNat, xs, init) >= x
-    {
-        if xs == [] {
+  function tcount(z: int, tys: seq<(int, nat)>): nat {
+    scount(z, Map((x: (int, nat)) => x.0, tys), (a,b) => a < b)
+  }
 
-        }else if |xs| == 1 {
-
-        }else{
-            assert xs == [xs[0]] + xs[1..];
-
-        }
-    }
-
-    lemma LemmaMaximum(xs: seq<nat>)
-        requires |xs| > 0
-        ensures forall x:: x in xs ==> maximum(xs) >= x
-    {
-        if |xs| == 1{
-
-        }else{
-            LemmaFoldRightMax(xs, xs[0]);
-        }
-    }
-
-    function msc(xs: seq<int>): nat 
-        requires |xs| > 1
-    {
-        var zzs := Map((zs) => assume |zs| > 0;
-            scount(zs[0], zs[1..], (a,b)=> a < b), Filter(xxs => |xxs| > 0, Tails(xs)));
-        maximum(zzs)
-    }
-
-    function table(xs: seq<int>): seq<(int, nat)>
-        requires |xs| > 1
-    {
-        Map((zs) => assume |zs| > 0;
-            (zs[0], scount(zs[0], zs[1..], (a,b)=> a < b)), Filter(xxs => |xxs| > 0, Tails(xs)))
-    }
-
-    function tcount(z: int, tys: seq<(int, nat)>): nat {
-        scount(z, Map((x: (int, nat)) => x.0, tys), (a,b) => a < b)
-    }
-
-    function join(txs: seq<(int, nat)>, tys: seq<(int, nat)>): seq<(int, nat)> {
-        Map((zc: (int,nat)) =>(zc.0, zc.1+tcount(zc.0, tys)), txs)+tys
-    }
+  function join(txs: seq<(int, nat)>, tys: seq<(int, nat)>): seq<(int, nat)> {
+    Map((zc: (int,nat)) =>(zc.0, zc.1+tcount(zc.0, tys)), txs)+tys
+  }
 }
